Proved theorems relating pushouts with coproducts and coequalizers. Proved that coequalizers are unique up to unique isomorphism using duality. Proved some other uniqueness properties for coequalizers. Put Set Implicit Arguments in a few places. Refactored uniqueness theorems for exponentials a bit. Proved a uniqueness theorem for exponentials involving classes. Moved non-skolemized definitions of exponentials to a separate file.

Exponential.v
@@ -4,11 +4,6 @@ Require Export Cat.
 Require Export InitTerm.
 Require Export BinProdCoprod.
 
-Definition exponential {C : Cat} {hp : has_products C}
-  (X Y E : Ob C) (eval : Hom (prodOb E X) Y) : Prop :=
-    forall (Z : Ob C) (e : Hom (prodOb Z X) Y),
-      exists!! u : Hom Z E, ProductFunctor_fmap u (id X) .> eval == e.
-
 Definition exponential_skolem {C : Cat} {hp : has_products C}
   (X Y E : Ob C) (eval : Hom (prodOb E X) Y)
   (curry : forall E' : Ob C, Hom (prodOb E' X) Y -> Hom E' E) : Prop :=
@@ -117,76 +112,14 @@ match goal with
     | |- ?x == ?x => reflexivity
 end.
 
-Theorem exponential_iso :
-    forall (C : Cat) (hp : has_products C) (X Y : Ob C)
-    (E : Ob C) (eval : Hom (prodOb E X) Y)
-    (E' : Ob C) (eval' : Hom (prodOb E' X) Y),
-        exponential X Y E eval -> exponential X Y E' eval' -> E ~ E'.
-Proof.
-  intros. red in H, H0.
-  destruct (H0 E eval0) as [u [Hu1 Hu2]], (H E' eval') as [u' [Hu'1 Hu'2]].
-  exists u, u'. split.
-    destruct (H E eval0) as [f [Hf1 Hf2]].
-    assert (f == id E).
-      apply Hf2. rewrite ProductFunctor_fmap_pres_id, id_left. reflexivity.
-      rewrite <- H1. symmetry. apply Hf2.
-        rewrite <- Hu'1, <- comp_assoc,
-        <- ProductFunctor_fmap_pres_comp in Hu1.
-        assert (ProductFunctor_fmap (u .> u') (id X .> id X)
-          == ProductFunctor_fmap (u .> u') (id X)).
-          apply ProductFunctor_fmap_Proper; auto. reflexivity.
-          rewrite H2 in Hu1. assumption.
-    destruct (H0 E' eval') as [f [Hf1 Hf2]].
-    assert (f == id E').
-      apply Hf2. rewrite ProductFunctor_fmap_pres_id, id_left. reflexivity.
-      rewrite <- H1. symmetry. apply Hf2.
-        rewrite <- Hu1, <- comp_assoc,
-        <- ProductFunctor_fmap_pres_comp in Hu'1.
-        assert (ProductFunctor_fmap (u' .> u) (id X .> id X)
-          == ProductFunctor_fmap (u' .> u) (id X)).
-          apply ProductFunctor_fmap_Proper; auto. reflexivity.
-          rewrite H2 in Hu'1. assumption.
-Defined.
-
-Theorem exponential_skolem_unique_long :
-    forall (C : Cat) (hp : has_products C) (X Y : Ob C)
-    (E : Ob C) (eval : Hom (prodOb E X) Y)
-      (curry : forall Z : Ob C, Hom (prodOb Z X) Y -> Hom Z E)
-    (E' : Ob C) (eval' : Hom (prodOb E' X) Y)
-      (curry' : forall Z : Ob C, Hom (prodOb Z X) Y -> Hom Z E'),
-        exponential_skolem X Y E eval curry ->
-        exponential_skolem X Y E' eval' curry'
-        -> E ~ E'.
-Proof.
-  intros. red. do 2 red in H. do 2 red in H0.
-  exists (curry' E eval0). red. exists (curry0 E' eval').
-  split.
-    destruct (H E eval0) as [H1 H2].
-      rewrite <- (H2 (curry' E eval0 .> curry0 E' eval')).
-        rewrite (H2 (id E)).
-          reflexivity.
-          rewrite ProductFunctor_fmap_pres_id, id_left. reflexivity.
-        rewrite ProductFunctor_fmap_pres_comp_l.
-          destruct (H E' eval'), (H0 E eval0).
-            rewrite comp_assoc. rewrite H3. rewrite H5. reflexivity.
-    destruct (H0 E' eval') as [H1 H2].
-      rewrite <- (H2 (curry0 E' eval' .> curry' E eval0)).
-        rewrite (H2 (id E')).
-          reflexivity.
-          rewrite ProductFunctor_fmap_pres_id, id_left. reflexivity.
-        rewrite ProductFunctor_fmap_pres_comp_l.
-          destruct (H E' eval'), (H0 E eval0).
-            rewrite comp_assoc. rewrite H5. rewrite H3. reflexivity.
-Qed.
-
 Theorem exponential_skolem_uiso :
   forall (C : Cat) (hp : has_products C) (X Y : Ob C)
   (E : Ob C) (eval : Hom (prodOb E X) Y)
   (curry : forall Z : Ob C, Hom (prodOb Z X) Y -> Hom Z E)
   (E' : Ob C) (eval' : Hom (prodOb E' X) Y)
   (curry' : forall Z : Ob C, Hom (prodOb Z X) Y -> Hom Z E'),
-      exponential_skolem X Y E eval curry ->
-      exponential_skolem X Y E' eval' curry' ->
+    exponential_skolem X Y E eval curry ->
+    exponential_skolem X Y E' eval' curry' ->
       exists !! f : Hom E E', Iso f /\
         f ×' id X .> eval' == eval.
 Proof.
@@ -215,13 +148,31 @@ Proof.
       apply ProductFunctor_fmap_Proper; cat. rewrite H3; cat.
 Qed.
 
-(* TODO *) Theorem has_exponentials_unique :
-  forall (C : Cat) (hp : has_products C) (hp' : has_products C)
-    (he : has_exponentials C) (he' : has_exponentials C) (X Y : Ob C),
-      @expOb C hp he X Y ~ @expOb C hp' he' X Y.
+Arguments exponential_skolem_uiso [C hp X Y E eval curry E' eval' curry'] _ _.
+
+Theorem exponential_skolem_iso :
+  forall (C : Cat) (hp : has_products C) (X Y : Ob C)
+  (E : Ob C) (eval : Hom (prodOb E X) Y)
+  (curry : forall Z : Ob C, Hom (prodOb Z X) Y -> Hom Z E)
+  (E' : Ob C) (eval' : Hom (prodOb E' X) Y)
+  (curry' : forall Z : Ob C, Hom (prodOb Z X) Y -> Hom Z E'),
+    exponential_skolem X Y E eval curry ->
+    exponential_skolem X Y E' eval' curry' ->
+      E ~ E'.
+Proof.
+  intros. destruct (exponential_skolem_uiso H H0). cat.
+Qed.
+
+Theorem has_exponentials_unique :
+  forall (C : Cat) (hp : has_products C)
+  (he : has_exponentials C) (he' : has_exponentials C) (X Y : Ob C),
+      @expOb C hp he X Y ~ @expOb C hp he' X Y.
 Proof.
   intros. destruct he, he'. simpl in *.
-Abort.
+  destruct (exponential_skolem_uiso
+    (is_exponential0 X Y) (is_exponential1 X Y)).
+  cat.
+Qed.
 
 Instance ExponentialFunctor
   (C : Cat) (hp : has_products C) (he : has_exponentials C)
