OldExponential.v
@@ -1,0 +1,41 @@
+Add Rec LoadPath "/home/zeimer/Code/Coq".
+
+Require Export Cat.
+Require Export InitTerm.
+Require Export BinProdCoprod.
+
+Definition exponential {C : Cat} {hp : has_products C}
+  (X Y E : Ob C) (eval : Hom (prodOb E X) Y) : Prop :=
+    forall (Z : Ob C) (e : Hom (prodOb Z X) Y),
+      exists!! u : Hom Z E, ProductFunctor_fmap u (id X) .> eval == e.
+
+Theorem exponential_iso :
+    forall (C : Cat) (hp : has_products C) (X Y : Ob C)
+    (E : Ob C) (eval : Hom (prodOb E X) Y)
+    (E' : Ob C) (eval' : Hom (prodOb E' X) Y),
+        exponential X Y E eval -> exponential X Y E' eval' -> E ~ E'.
+Proof.
+  intros. red in H, H0.
+  destruct (H0 E eval0) as [u [Hu1 Hu2]], (H E' eval') as [u' [Hu'1 Hu'2]].
+  exists u, u'. split.
+    destruct (H E eval0) as [f [Hf1 Hf2]].
+    assert (f == id E).
+      apply Hf2. rewrite ProductFunctor_fmap_pres_id, id_left. reflexivity.
+      rewrite <- H1. symmetry. apply Hf2.
+        rewrite <- Hu'1, <- comp_assoc,
+        <- ProductFunctor_fmap_pres_comp in Hu1.
+        assert (ProductFunctor_fmap (u .> u') (id X .> id X)
+          == ProductFunctor_fmap (u .> u') (id X)).
+          apply ProductFunctor_fmap_Proper; auto. reflexivity.
+          rewrite H2 in Hu1. assumption.
+    destruct (H0 E' eval') as [f [Hf1 Hf2]].
+    assert (f == id E').
+      apply Hf2. rewrite ProductFunctor_fmap_pres_id, id_left. reflexivity.
+      rewrite <- H1. symmetry. apply Hf2.
+        rewrite <- Hu1, <- comp_assoc,
+        <- ProductFunctor_fmap_pres_comp in Hu'1.
+        assert (ProductFunctor_fmap (u' .> u) (id X .> id X)
+          == ProductFunctor_fmap (u' .> u) (id X)).
+          apply ProductFunctor_fmap_Proper; auto. reflexivity.
+          rewrite H2 in Hu'1. assumption.
+Defined.
