README.md
@@ -26,6 +26,8 @@ General TODO:
  * Refactor the products and coproducts — put them in separate files in a new directory. Make a new file about finite (and not just binary) products/coproducts and put there the theorems that relate binary products/coproducts with initial and terminal objects.
  * Port all properties of universal constructions to skolemized definitions.
  * Use more duality.
+ * Use Set Implicit Arguments more.
+ * Prove more properties of universal constructions (like these for equalizers).
 
 Instances:
  * Solve the dependent type problems with setoid coproducts.
